src/tls/KeySchedule.fst
@@ -20,6 +20,8 @@ open Range
 open HandshakeMessages
 open StatefulLHAE
 open HKDF
+open Negotiation // We only depend minimally on Nego
+open Epochs	 // We only depend minimally on Epochs 
 
 // KEF.fst/TLSPRF.fst for TLS 1.2
 // CoreCrypto.hkdf for TLS 1.3
@@ -737,3 +739,96 @@ let ks_client_12_server_verify_data ks log =
   st := C C_Done;
   TLSPRF.verifyData (pv,cs) ms Server log
 
+
+val getId: recordInstance -> GTot id
+let getId k = 
+    match k with
+    | StAEInstance #i rd wr -> i
+    | StLHAEInstance #i rd wr -> i
+
+#set-options "--lax"
+
+val recordInstanceToEpoch: #r:rgn -> #n:TLSInfo.random -> 
+    			   h:handshake ->
+			   ks:recordInstance -> Tot (epoch r n)
+let recordInstanceToEpoch #hs_rgn #n hs ri = 
+    match ri with
+    | StAEInstance #i rd wr -> Epoch hs (StAE.Stream () rd) (StAE.Stream () wr)
+    | StLHAEInstance #i rd wr -> Epoch hs (StAE.StLHAE () rd) (StAE.StLHAE () wr)
+
+
+(*
+let id_TLS12_AES_GCM_128_SHA256  = {
+    msId = noMsId;
+    kdfAlg = PRF_TLS_1p2 kdf_label (HMAC CoreCrypto.SHA256);
+    pv = TLS_1p2;
+    aeAlg = (AEAD CoreCrypto.AES_128_GCM CoreCrypto.SHA256);
+    csrConn = createBytes 64 0x00z;
+    ext = {
+      ne_extended_ms = false;
+      ne_extended_padding = false;
+      ne_secure_renegotiation = RI_Unsupported;
+      ne_supported_groups = None;
+      ne_supported_point_formats = None;
+      ne_server_names = None;
+      ne_signature_algorithms = None;
+      ne_keyShare = None;
+    };
+    writer = Client
+  }
+
+val encryptor_TLS12_AES_GCM_128_SHA256: hs:handshake -> bytes -> bytes -> ST (StAE.writer (hsId hs))
+  (requires (fun h -> True))
+  (ensures (fun h0 i h1 -> True))
+let encryptor_TLS12_AES_GCM_128_SHA256 hs key iv = 
+  let id = hsId hs in
+  let r = HyperHeap.root in
+  let w: StatefulLHAE.writer id =
+    let log: StatefulLHAE.st_log_t r id = ralloc r Seq.createEmpty in
+    let seqn: HyperHeap.rref r seqn_t = ralloc r 0 in
+    let key: AEAD_GCM.state id Writer =
+      // The calls to [unsafe_coerce] are here because we're breaking
+      // abstraction, as both [key] and [iv] are declared as private types.
+      let key: AEAD_GCM.key id = key |> unsafe_coerce in
+      let iv: AEAD_GCM.iv id = iv |> unsafe_coerce in
+      let log: HyperHeap.rref r _ = ralloc r Seq.createEmpty in
+      let counter = ralloc r 0 in
+      AEAD_GCM.State r key iv log counter
+    in
+    StatefulLHAE.State r log seqn key
+  in
+  // StatefulLHAE.writer -> StatefulLHAE.state
+  StAE.StLHAE () w
+
+val decryptor_TLS12_AES_GCM_128_SHA256: hs:handshake -> bytes -> bytes -> ST (StAE.reader (peerId (hsId hs)))
+  (requires (fun h -> True))
+  (ensures (fun h0 i h1 -> True))
+let decryptor_TLS12_AES_GCM_128_SHA256 hs key iv = 
+  let id = peerId (hsId hs) in
+  let r = HyperHeap.root in
+  let r: StatefulLHAE.reader id =
+    let log: StatefulLHAE.st_log_t r id = ralloc r Seq.createEmpty in
+    let seqn: HyperHeap.rref r seqn_t = ralloc r 0 in
+    let key: AEAD_GCM.state id Reader =
+      // The calls to [unsafe_coerce] are here because we're breaking
+      // abstraction, as both [key] and [iv] are declared as private types.
+      let key: AEAD_GCM.key id = key |> unsafe_coerce in
+      let iv: AEAD_GCM.iv id = iv |> unsafe_coerce in
+      let log: HyperHeap.rref r _ = ralloc r Seq.createEmpty in
+      let counter = ralloc r 0 in
+      AEAD_GCM.State r key iv log counter
+    in
+    StatefulLHAE.State r log seqn key
+  in
+  // StatefulLHAE.reader -> StatefulLHAE.state
+  StAE.StLHAE () r
+
+val recordKeysToEpoch: #hs_rgn:rgn -> #n:TLSInfo.random -> h:handshake -> (bytes * bytes * bytes * bytes) -> ST (epoch hs_rgn n)
+  (requires (fun h -> True))
+  (ensures (fun h0 i h1 -> True))
+let recordKeysToEpoch #hs_rgn #n h (ck,civ,sk,siv) = 
+  let wr: StAE.writer (hsId h) = encryptor_TLS12_AES_GCM_128_SHA256 h ck civ in
+  let rd: StAE.reader (peerId (hsId h)) = decryptor_TLS12_AES_GCM_128_SHA256 h sk siv in
+  Epoch h rd wr
+
+*)
