src/tls/Epochs.fst
@@ -1,0 +1,136 @@
+module Epochs
+open FStar.Heap
+open FStar.HyperHeap
+open FStar.Seq
+open FStar.SeqProperties // for e.g. found
+open FStar.Set  
+open Platform.Error
+open Platform.Bytes
+
+open TLSError
+open TLSInfo
+open TLSConstants
+open Range
+open HandshakeMessages
+open StAE
+open Negotiation
+
+// relocate?
+type fresh_subregion r0 r h0 h1 = fresh_region r h0 h1 /\ extends r r0
+
+type epoch_region_inv (#i:id) (hs_rgn:rgn) (r:reader (peerId i)) (w:writer i) =
+  disjoint hs_rgn (region w)                  /\
+  parent (region w) <> FStar.HyperHeap.root    /\
+  parent (region r) <> FStar.HyperHeap.root    /\
+  parent hs_rgn = parent (parent (region w))  /\ //Grandparent of each writer is a sibling of the handshake
+  disjoint (region w) (region r)              /\
+  is_epoch_rgn (region w)                     /\ //they're all colored as epoch regions
+  is_epoch_rgn (region r)                     /\
+  is_epoch_rgn (parent (region w))            /\
+  is_epoch_rgn (parent (region r))            /\
+  is_hs_rgn hs_rgn                              //except for the hs_rgn, of course
+
+abstract type epoch_region_inv' (#i:id) (hs_rgn:rgn) (r:reader (peerId i)) (w:writer i) =
+  epoch_region_inv hs_rgn r w
+
+module I = IdNonce
+
+type epoch (hs_rgn:rgn) (n:TLSInfo.random) = 
+  | Epoch: h:handshake -> 
+    	   #i: id ->
+           r: reader (peerId i) ->
+           w: writer i {epoch_region_inv' hs_rgn r w /\ I.nonce_of_id i = n} 
+	   -> epoch hs_rgn n
+  // we would extend/adapt it for TLS 1.3,
+  // e.g. to notify 0RTT/forwad-privacy transitions
+  // for now epoch completion is a total function on handshake --- should be stateful
+
+
+let reveal_epoch_region_inv_all (u:unit)
+  : Lemma (forall i hs_rgn r w.{:pattern (epoch_region_inv' #i hs_rgn r w)}
+	   epoch_region_inv' #i hs_rgn r w
+	   <==>
+   	   epoch_region_inv #i hs_rgn r w)
+  = ()	   
+
+let reveal_epoch_region_inv (#hs_rgn:rgn) (#n:TLSInfo.random) (e:epoch hs_rgn n) 
+  : Lemma (let r = Epoch.r e in 
+	   let w = Epoch.w e in 
+	   epoch_region_inv hs_rgn r w)
+  = ()
+
+let writer_epoch (#hs_rgn:rgn) (#n:TLSInfo.random) (e:epoch hs_rgn n) 
+  : Tot (w:writer (hsId (e.h)) {epoch_region_inv hs_rgn (Epoch.r e) w})
+  = Epoch.w e
+
+let reader_epoch (#hs_rgn:rgn) (#n:TLSInfo.random) (e:epoch hs_rgn n) 
+  : Tot (r:reader (peerId (hsId (e.h))) {epoch_region_inv hs_rgn r (Epoch.w e)})
+  = match e with | Epoch hs #i r w -> r //16-05-20 Epoch.r e failed.
+
+(* The footprint just includes the writer regions *)
+abstract let epochs_inv (#r:rgn) (#n:TLSInfo.random) (es: seq (epoch r n)) =
+  forall (i:nat { i < Seq.length es })
+    (j:nat { j < Seq.length es /\ i <> j}).{:pattern (Seq.index es i); (Seq.index es j)}
+    let ei = Seq.index es i in
+    let ej = Seq.index es j in
+    parent (region ei.w) = parent (region ej.w) /\  //they all descend from a common epochs sub-region of the connection
+    disjoint (region ei.w) (region ej.w)           //each epoch writer lives in a region disjoint from the others
+
+abstract let epochs_inv' (#r:rgn) (#n:TLSInfo.random) (es: seq (epoch r n)) = epochs_inv es
+
+let reveal_epochs_inv' (u:unit)
+  : Lemma (forall (r:rgn) (#n:TLSInfo.random) (es:seq (epoch r n)). {:pattern (epochs_inv' es)}
+	     epochs_inv' es
+	     <==>
+	     epochs_inv es)
+  = ()
+
+
+type epochs (r:rgn) (n:TLSInfo.random) = 
+  | Epochs: es: MonotoneSeq.i_seq r (epoch r n) epochs_inv -> 
+    	    read: rref r int -> 
+	    write: rref r int ->
+	    epochs r n  
+// idx must be between -1 and Seq.length (!es) -1 (inclusive)
+
+let containsT (Epochs es r w) (h:HyperHeap.t) =
+    MonotoneSeq.i_contains es h 
+
+val epochs_init: r:rgn -> n:TLSInfo.random -> ST (epochs r n)
+       (requires (fun h -> True))
+       (ensures (fun h0 x h1 -> True))
+let epochs_init (r:rgn) (n:TLSInfo.random) = 
+    let esref = MonotoneSeq.alloc_mref_seq r Seq.createEmpty in
+    let rref = ralloc r (-1) in
+    let wref = ralloc r (-1) in
+    Epochs esref rref wref
+
+val add_epoch: #r:rgn -> #n:TLSInfo.random -> 
+    	       es:epochs r n -> e: epoch r n -> ST unit
+       (requires (fun h -> True))
+       (ensures (fun h0 x h1 -> True))
+let add_epoch #rg #n (Epochs es r w) e = 
+    MonotoneSeq.i_write_at_end #rg es e
+
+val set_reader: #r:rgn -> #n:TLSInfo.random -> 
+    	       es:epochs r n -> i:nat -> ST unit
+       (requires (fun h -> True))
+       (ensures (fun h0 x h1 -> True))
+let set_reader #r #n (Epochs es r w) i' = r := i'
+
+
+val set_writer: #r:rgn -> #n:TLSInfo.random -> 
+    	       es:epochs r n -> i:nat -> ST unit
+       (requires (fun h -> True))
+       (ensures (fun h0 x h1 -> True))
+let set_writer #r #n (Epochs es r w) i' = w := i'
+
+let get_epochs (Epochs es r w) = es 
+
+let epochsT (Epochs es r w) (h:HyperHeap.t) = MonotoneSeq.i_sel h es
+
+let readerT (Epochs es r w) (h:HyperHeap.t) = sel h r
+
+let writerT (Epochs es r w) (h:HyperHeap.t) = sel h w
+
+
