src/tls/Negotiation.fst
@@ -1,0 +1,59 @@
+module Negotiation
+
+open Platform.Error
+open Platform.Bytes
+
+open TLSError
+open TLSInfo
+open TLSConstants
+open HandshakeMessages
+
+//16-05-31 these opens are implementation-only; overall we should open less
+open TLSExtensions 
+open CoreCrypto
+
+(* Negotiation: HELLO sub-module *)
+type ri = cVerifyData * sVerifyData 
+
+type nego = {
+     n_resume: bool;
+     n_client_random: TLSInfo.random;
+     n_server_random: TLSInfo.random;
+     n_sessionID: option sessionID;
+     n_protocol_version: protocolVersion;
+     n_kexAlg: TLSConstants.kexAlg;
+     n_aeAlg: TLSConstants.aeAlg;
+     n_sigAlg: option TLSConstants.sigAlg;
+     n_cipher_suite: cipherSuite;
+     n_dh_group: option namedGroup;
+     n_compression: option compression;
+     n_extensions: negotiatedExtensions;
+     n_scsv: list scsv_suite;
+}                 
+
+type hs_id = {
+     id_cert: Cert.chain;
+     id_sigalg: option sigHashAlg;
+}
+
+type session = {
+     session_nego: nego;
+}     
+
+
+// represents the outcome of a successful handshake, 
+// providing context for the derived epoch
+type handshake = 
+  | Fresh of session // was sessionInfo
+  | Resumed of session // was abbrInfo * sessionInfo 
+// We use SessionInfo as unique session indexes.
+// We tried using instead hs, but this creates circularities
+// We'll probably need a global log to reason about them.
+// We should probably do the same in the session store.
+
+// extracts a transport key identifier from a handshake record
+val hsId: handshake -> Tot id 
+//16-05-31 TODO breaking TC in TLS; was (i:id { is_stream_ae i }) //16-05-19 focus on TLS 1.3
+
+let hsId h = noId // Placeholder 
+
